Refine syntactic relation for known-correctness
Still problematic, mostly because the syntactic connection between two
expressions (the bodies of closures) depends on
parameters (environmental approximation and approximation information
for globals), and it seems as if these parameters have to appear as
parameters to the relation; then they vary in the inductive hypotheses.

Handling the way the environment approximation changes in evaluating Let
is the current stumbling block.

compiler/backend/proofs/clos_knownProofScript.sml
@@ -1354,24 +1354,31 @@ val evaluate_app_NONE_SOME = Q.store_thm(
   rpt (pairarg_tac >> fs[]) >> rveq >>
   fs[check_loc_def, revdroprev, revtakerev]);
 
-val _ = new_constant("kvrel", ``:closSem$v -> closSem$v -> bool``)
+val kerel_def = Define`
+  kerel as g0 e1 e2 ⇔
+    e1 = e2 ∨
+    ∃a as' g0' g'.
+      better_definedg g0' g0 ∧ as' <<= as ∧ known [e1] as' g0' = ([(e2,a)], g')
+`;
 
 val kvrel_def = tDefine "kvrel" `
-  (kvrel (Number i) v ⇔ v = Number i) ∧
-  (kvrel (Word64 w) v ⇔ v = Word64 w) ∧
-  (kvrel (Block n vs) v ⇔ ∃vs'. v = Block n vs' ∧ LIST_REL kvrel vs vs') ∧
-  (kvrel (RefPtr n) v ⇔ v = RefPtr n) ∧
-  (kvrel (Closure lopt vs1 vs2 n bod) v ⇔
+  (kvrel as g (Number i) v ⇔ v = Number i) ∧
+  (kvrel as g (Word64 w) v ⇔ v = Word64 w) ∧
+  (kvrel as g (Block n vs) v ⇔
+     ∃vs'. v = Block n vs' ∧ LIST_REL (kvrel as g) vs vs') ∧
+  (kvrel as g (RefPtr n) v ⇔ v = RefPtr n) ∧
+  (kvrel as g (Closure lopt vs1 vs2 n bod) v ⇔
      ∃vs1' vs2' bod'.
-       LIST_REL kvrel vs1 vs1' ∧ LIST_REL kvrel vs2 vs2' ∧
-       set_globals bod = set_globals bod' ∧ v = Closure lopt vs1' vs2' n bod') ∧
-  (kvrel (Recclosure lopt vs1 vs2 fns i) v ⇔
+       LIST_REL (kvrel as g) vs1 vs1' ∧ LIST_REL (kvrel as g) vs2 vs2' ∧
+       kerel as g bod bod' ∧
+       v = Closure lopt vs1' vs2' n bod') ∧
+  (kvrel as g (Recclosure lopt vs1 vs2 fns i) v ⇔
      ∃vs1' vs2' fns'.
-       LIST_REL kvrel vs1 vs1' ∧ LIST_REL kvrel vs2 vs2' ∧
-       LIST_REL (λ(n1,e1) (n2,e2). n1 = n2 ∧ set_globals e1 = set_globals e2)
+       LIST_REL (kvrel as g) vs1 vs1' ∧ LIST_REL (kvrel as g) vs2 vs2' ∧
+       LIST_REL (λ(n1,e1) (n2,e2). n1 = n2 ∧ kerel as g e1 e2)
                 fns fns' ∧
-        v = Recclosure lopt vs1' vs2' fns' i)
-` (WF_REL_TAC `measure (v_size o FST)` >> simp[v_size_def] >>
+       v = Recclosure lopt vs1' vs2' fns' i)
+` (WF_REL_TAC `measure (v_size o FST o SND o SND)` >> simp[v_size_def] >>
    rpt strip_tac >> imp_res_tac v_size_lemma >> simp[])
 val kvrel_ind = theorem "kvrel_ind"
 val kvrel_def = save_thm(
@@ -1381,42 +1388,67 @@ val kvrel_def = save_thm(
 (* necessary kvrel *)
 val kvrel_vsgc_free = Q.store_thm(
   "kvrel_vsgc_free",
-  `∀v1 v2. kvrel v1 v2 ⇒ (vsgc_free v1 ⇔ vsgc_free v2)`,
+  `∀as g v1 v2. kvrel as g v1 v2 ⇒ (vsgc_free v1 ⇔ vsgc_free v2)`,
   ho_match_mp_tac kvrel_ind >> simp[] >> rpt strip_tac
   >- (fs[EVERY_MEM, LIST_REL_EL_EQN] >> metis_tac[MEM_EL])
-  >- (fs[EVERY_MEM, LIST_REL_EL_EQN] >> metis_tac[MEM_EL])
+  >- (fs[EVERY_MEM, LIST_REL_EL_EQN] >>
+      fs[kerel_def] >- metis_tac[MEM_EL] >>
+      imp_res_tac known_preserves_setGlobals >>
+      fs[] >> metis_tac[MEM_EL])
   >- (fs[EVERY_MEM, LIST_REL_EL_EQN, elglobals_EQ_EMPTY, MEM_MAP, PULL_EXISTS,
          FORALL_PROD]>>
       EQ_TAC >> rpt strip_tac
       >- (imp_res_tac (MEM_EL |> SPEC_ALL |> EQ_IMP_RULE |> #1 |> GSYM) >>
           qcase_tac `m < LENGTH fns'` >>
           Cases_on `EL m fns` >> fs[] >>
-          first_x_assum (qspec_then `m` mp_tac) >> simp[] >> metis_tac[MEM_EL])
+          first_x_assum (qspec_then `m` mp_tac) >> simp[] >>
+          rw[kerel_def] >- metis_tac[MEM_EL] >>
+          imp_res_tac known_preserves_setGlobals >> fs[] >>
+          metis_tac[MEM_EL])
       >- metis_tac[MEM_EL]
       >- metis_tac[MEM_EL]
       >- (imp_res_tac (MEM_EL |> SPEC_ALL |> EQ_IMP_RULE |> #1 |> GSYM) >>
           qcase_tac `m < LENGTH fns` >>
           Cases_on `EL m fns'` >> fs[] >>
-          first_x_assum (qspec_then `m` mp_tac) >> simp[] >> metis_tac[MEM_EL])
+          first_x_assum (qspec_then `m` mp_tac) >> simp[] >>
+          rw[kerel_def] >- metis_tac[MEM_EL] >>
+          imp_res_tac known_preserves_setGlobals >> fs[] >>
+          metis_tac[MEM_EL])
       >- metis_tac[MEM_EL]
       >- metis_tac[MEM_EL]))
 
+(* necessary kvrel *)
+val kvrel_approx_prefix = Q.store_thm(
+  "kvrel_approx_prefix",
+  `∀as0 g v1 v2 as1. kvrel as0 g v1 v2 ∧ as0 <<= as1 ⇒ kvrel as1 g v1 v2`,
+  ho_match_mp_tac kvrel_ind >> simp[] >> rpt strip_tac
+  >- (fs[LIST_REL_EL_EQN] >> metis_tac[MEM_EL])
+  >- (fs[LIST_REL_EL_EQN] >> reverse (rpt conj_tac)
+      >- (fs[kerel_def] >> metis_tac[IS_PREFIX_TRANS]) >> metis_tac[MEM_EL])
+  >- (fs[LIST_REL_EL_EQN] >> reverse (rpt conj_tac)
+      >- (qx_gen_tac `j` >> rfs[] >> strip_tac >> res_tac >>
+          rpt (pairarg_tac >> fs[]) >> fs[kerel_def] >>
+          metis_tac[IS_PREFIX_TRANS]) >>
+      metis_tac[MEM_EL]))
+
 val kvrel_Boolv = Q.store_thm(
   "kvrel_Boolv[simp]",
-  `(kvrel (Boolv b) v ⇔ v = Boolv b) ∧
-   (kvrel v (Boolv b) ⇔ v = Boolv b)`,
+  `(kvrel as g (Boolv b) v ⇔ v = Boolv b) ∧
+   (kvrel as g v (Boolv b) ⇔ v = Boolv b)`,
   simp[closSemTheory.Boolv_def] >> Cases_on `v` >> simp[] >> metis_tac[]);
 
 val kvrel_EVERY_vsgc_free = Q.store_thm(
   "kvrel_EVERY_vsgc_free",
   `∀vs1 vs2.
-     LIST_REL kvrel vs1 vs2 ⇒ (EVERY vsgc_free vs1 ⇔ EVERY vsgc_free vs2)`,
+     LIST_REL (kvrel as g) vs1 vs2 ⇒
+     (EVERY vsgc_free vs1 ⇔ EVERY vsgc_free vs2)`,
   Induct_on `LIST_REL` >> simp[] >> metis_tac[kvrel_vsgc_free]);
 
 (* necessary kvrel *)
 val kvrel_val_approx = Q.store_thm(
   "kvrel_val_approx",
-  `∀v1 v2. kvrel v1 v2 ⇒ ∀a. val_approx_val a v1 ⇔ val_approx_val a v2`,
+  `∀as g v1 v2.
+     kvrel as g v1 v2 ⇒ ∀a. val_approx_val a v1 ⇔ val_approx_val a v2`,
   ho_match_mp_tac kvrel_ind >> rw[]
   >- (Cases_on `a` >> simp[] >> fs[LIST_REL_EL_EQN] >> metis_tac[MEM_EL])
   >- (Cases_on `a` >> simp[] >> fs[LIST_REL_EL_EQN] >> metis_tac[LENGTH_NIL])
@@ -1431,7 +1463,7 @@ val kvrel_val_approx = Q.store_thm(
 val kvrel_LIST_REL_val_approx = Q.store_thm(
   "kvrel_LIST_REL_val_approx",
   `∀vs1 vs2.
-      LIST_REL kvrel vs1 vs2 ⇒
+      LIST_REL (kvrel as g) vs1 vs2 ⇒
       ∀as. LIST_REL val_approx_val as vs1 ⇔ LIST_REL val_approx_val as vs2`,
   Induct_on `LIST_REL` >> simp[] >> metis_tac[kvrel_val_approx]);
 
@@ -1454,49 +1486,75 @@ val ksrel_ssgc_free = Q.store_thm(
   simp[ksrel_def]);
 
 val krrel_def = Define`
-  (krrel (Rval vs1, s1) r ⇔
-      ∃s2 vs2. r = (Rval vs2,s2) ∧ LIST_REL kvrel vs1 vs2 ∧ ksrel s1 s2) ∧
-  (krrel (Rerr (Rabort Rtype_error), _) _ ⇔ T) ∧
-  (krrel (Rerr (Rabort Rtimeout_error), s1) (Rerr e, s2) ⇔
+  (krrel as g (Rval vs1, s1) r ⇔
+      ∃s2 vs2. r = (Rval vs2,s2) ∧ LIST_REL (kvrel as g) vs1 vs2 ∧
+               ksrel s1 s2) ∧
+  (krrel as g (Rerr (Rabort Rtype_error), _) _ ⇔ T) ∧
+  (krrel as g (Rerr (Rabort Rtimeout_error), s1) (Rerr e, s2) ⇔
      e = Rabort Rtimeout_error ∧ ksrel s1 s2) ∧
-  (krrel (Rerr (Rraise v1), s1) (Rerr (Rraise v2), s2) ⇔
-     kvrel v1 v2 ∧ ksrel s1 s2) ∧
-  (krrel _ _ ⇔ F)
+  (krrel as g (Rerr (Rraise v1), s1) (Rerr (Rraise v2), s2) ⇔
+     kvrel as g v1 v2 ∧ ksrel s1 s2) ∧
+  (krrel _ _ _ _ ⇔ F)
 `;
 val _ = export_rewrites ["krrel_def"]
 
 val krrel_errval = Q.store_thm(
   "krrel_errval[simp]",
-  `(krrel (Rerr e, s1) (Rval vs, s2) ⇔ e = Rabort Rtype_error)`,
+  `(krrel as g (Rerr e, s1) (Rval vs, s2) ⇔ e = Rabort Rtype_error)`,
   Cases_on `e` >> simp[] >> qcase_tac `Rabort a` >> Cases_on `a` >> simp[]);
 
 val krrel_err_rw = Q.store_thm(
   "krrel_err_rw",
-  `krrel (Rerr e, s1) r ⇔
+  `krrel as g (Rerr e, s1) r ⇔
       e = Rabort Rtype_error ∨
       (∃s2. e = Rabort Rtimeout_error ∧ r = (Rerr (Rabort Rtimeout_error), s2) ∧
             ksrel s1 s2) ∨
       (∃v1 v2 s2.
-            e = Rraise v1 ∧ r = (Rerr (Rraise v2),s2) ∧ kvrel v1 v2 ∧
+            e = Rraise v1 ∧ r = (Rerr (Rraise v2),s2) ∧ kvrel as g v1 v2 ∧
             ksrel s1 s2)`,
   Cases_on `e` >> simp[] >> Cases_on `r` >> simp[]
-  >- (qcase_tac `krrel _ (r2, s2)` >> Cases_on `r2` >> simp[] >>
-      qcase_tac `krrel _ (Rerr e,_)` >> Cases_on `e` >> simp[])
+  >- (qcase_tac `krrel _ _ _ (r2, s2)` >> Cases_on `r2` >> simp[] >>
+      qcase_tac `krrel _ _ _ (Rerr e,_)` >> Cases_on `e` >> simp[])
   >- (qcase_tac `Rabort abt` >> Cases_on `abt` >> simp[] >>
-      qcase_tac `krrel _ (r2,s2)` >> Cases_on `r2` >> simp[]));
+      qcase_tac `krrel _ _ _ (r2,s2)` >> Cases_on `r2` >> simp[]));
+
+(* kvrel necessary *)
+val kvrel_better_definedg = Q.store_thm(
+  "kvrel_better_definedg",
+  `∀as g1 v1 v2 g2.
+     better_definedg g1 g2 ∧ kvrel as g1 v1 v2 ⇒ kvrel as g2 v1 v2`,
+  ho_match_mp_tac kvrel_ind >> simp[PULL_EXISTS] >> rpt strip_tac
+  >- (fs[LIST_REL_EL_EQN] >> metis_tac[MEM_EL])
+  >- (fs[LIST_REL_EL_EQN] >> metis_tac[MEM_EL])
+  >- (fs[LIST_REL_EL_EQN] >> metis_tac[MEM_EL])
+  >- (fs[kerel_def] >> metis_tac[better_definedg_trans])
+  >- (fs[LIST_REL_EL_EQN] >> metis_tac[MEM_EL])
+  >- (fs[LIST_REL_EL_EQN] >> metis_tac[MEM_EL])
+  >- (fs[LIST_REL_EL_EQN] >> rfs[] >> qx_gen_tac `j` >> strip_tac >>
+      res_tac >> rpt (pairarg_tac >> fs[]) >> fs[kerel_def] >>
+      metis_tac[better_definedg_trans]))
+
+(* krrel necessary *)
+val krrel_better_definedg = Q.store_thm(
+  "krrel_better_definedg",
+  `∀as g1 g2 res1 res2.
+     better_definedg g1 g2 ∧ krrel as g1 res1 res2 ⇒ krrel as g2 res1 res2`,
+  rpt gen_tac >> Cases_on `res1` >> Cases_on `res2` >>
+  qcase_tac `krrel as g1 (rv1, s1)` >> Cases_on `rv1` >>
+  dsimp[krrel_err_rw] >> metis_tac[LIST_REL_mono, kvrel_better_definedg]);
 
 (*
 val known_correct0 = Q.prove(
-  `(∀a es env1 env2 (s01:α closSem$state) s02 res1 s1 g0 g as ealist.
+  `(∀a es env1 env2 (s01:α closSem$state) s02 res1 s1 g0 g as eas ealist.
       a = (es,env1,s01) ∧ evaluate (es, env1, s01) = (res1, s1) ∧
-      EVERY esgc_free es ∧
+      EVERY esgc_free es ∧ eas <<= as ∧
       LIST_REL val_approx_val as env1 ∧ EVERY vsgc_free env1 ∧
-      LIST_REL kvrel env1 env2 ∧ ksrel s01 s02 ∧
+      LIST_REL (kvrel eas g0) env1 env2 ∧ ksrel s01 s02 ∧
       state_globals_approx s01 g0 ∧
       ssgc_free s01 ∧ known es as g0 = (ealist, g) ⇒
       ∃res2 s2.
         evaluate(MAP FST ealist, env2, s02) = (res2, s2) ∧
-        krrel (res1,s1) (res2,s2)) ∧
+        krrel as g (res1,s1) (res2,s2)) ∧
    (∀lopt f args (s0:α closSem$state) res s.
       evaluate_app lopt f args s0 = (res,s) ∧ EVERY vsgc_free args ⇒ T)`,
   ho_match_mp_tac evaluate_ind >> rpt conj_tac
@@ -1509,42 +1567,57 @@ val known_correct0 = Q.prove(
       >- (imp_res_tac evaluate_SING >> rveq >> fs[] >>
           imp_res_tac known_sing_EQ_E >> rveq >> fs[] >>
           simp[Once evaluate_CONS, pair_case_eq, result_case_eq, PULL_EXISTS] >>
-          sel_ihpc last >> simp[PULL_EXISTS] >>
-          disch_then irule >> simp[]
-          >- metis_tac[ssgc_free_preserved_SING']
-          >- (qpat_assum `known [_] _ _ = _`
-                 (mp_tac o MATCH_MP (GEN_ALL kca_sing_sga)) >> simp[] >>
-              strip_tac >> sel_ihpc last >> reverse impl_tac
-              >- metis_tac[ksrel_sga] >> simp[] >> rpt strip_tac
-              >- metis_tac[kvrel_LIST_REL_val_approx]
-              >- metis_tac[ksrel_sga]
-              >- metis_tac[ksrel_ssgc_free]
-              >- metis_tac[kvrel_EVERY_vsgc_free]))
+          sel_ihpc last >> simp[PULL_EXISTS] >> strip_tac >>
+          qcase_tac `LIST_REL (kvrel eas g0) env1 env2` >>
+          qcase_tac `known [exp1] as g0 = ([(exp2,apx1)], g1)` >>
+          qcase_tac `evaluate ([exp1],env1,s01) = (Rval [v01], s11)` >>
+          qcase_tac `evaluate ([exp2],env2,s02) = (Rval [v02], s12)` >>
+          first_x_assum (qspecl_then [`env2`, `s12`, `eas`] mp_tac) >> impl_tac
+          >- (simp[] >> rpt conj_tac
+              >- (irule LIST_REL_mono >> qexists_tac `kvrel eas g0` >>
+                  simp[] >>
+                  metis_tac[kvrel_better_definedg, known_better_definedg])
+              >- (qpat_assum `known [_] _ _ = _`
+                    (mp_tac o MATCH_MP (GEN_ALL kca_sing_sga)) >> simp[] >>
+                  strip_tac >> sel_ihpc last >> reverse impl_tac
+                  >- metis_tac[ksrel_sga] >> simp[] >> rpt strip_tac
+                  >- metis_tac[kvrel_LIST_REL_val_approx]
+                  >- metis_tac[ksrel_sga]
+                  >- metis_tac[ksrel_ssgc_free]
+                  >- metis_tac[kvrel_EVERY_vsgc_free])
+              >- metis_tac[ssgc_free_preserved_SING']) >>
+          metis_tac[kvrel_better_definedg, known_better_definedg])
       >- (imp_res_tac evaluate_SING >> rveq >> fs[] >>
           imp_res_tac known_sing_EQ_E >> rveq >> fs[] >>
           simp[Once evaluate_CONS, pair_case_eq, result_case_eq, PULL_EXISTS] >>
-          dsimp[] >> sel_ihpc last >> simp[] >>
-          strip_tac >> sel_ihpc hd >> simp[] >> strip_tac >> sel_ihpc hd >>
-          impl_tac
-          >- (simp[] >> reverse conj_tac
-              >- metis_tac[ssgc_free_preserved_SING']
+          dsimp[] >> sel_ihpc last >> simp[] >> strip_tac >>
+          qcase_tac `LIST_REL (kvrel eas g0) env1 env2` >>
+          qcase_tac `known [exp1] as g0 = ([(exp2,apx1)], g1)` >>
+          qcase_tac `evaluate ([exp1],env1,s01) = (Rval [v01], s11)` >>
+          qcase_tac `evaluate ([exp2],env2,s02) = (Rval [v02], s12)` >>
+          first_x_assum (qspecl_then [`env2`, `s12`, `eas`] mp_tac) >> impl_tac
+          >- (simp[] >> rpt conj_tac
+              >- (irule LIST_REL_mono >> qexists_tac `kvrel eas g0` >>
+                  simp[] >>
+                  metis_tac[kvrel_better_definedg, known_better_definedg])
               >- (qpat_assum `known [_] _ _ = _`
-                 (mp_tac o MATCH_MP (GEN_ALL kca_sing_sga)) >> simp[] >>
-                 strip_tac >> sel_ihpc last >> reverse impl_tac
-                 >- metis_tac[ksrel_sga] >> simp[] >> rpt strip_tac
-                 >- metis_tac[kvrel_LIST_REL_val_approx]
-                 >- metis_tac[ksrel_sga]
-                 >- metis_tac[ksrel_ssgc_free]
-                 >- metis_tac[kvrel_EVERY_vsgc_free])) >>
-          strip_tac >> simp[] >> fs[krrel_err_rw] >>
-          metis_tac[result_CASES])
+                    (mp_tac o MATCH_MP (GEN_ALL kca_sing_sga)) >> simp[] >>
+                  strip_tac >> sel_ihpc last >> reverse impl_tac
+                  >- metis_tac[ksrel_sga] >> simp[] >> rpt strip_tac
+                  >- metis_tac[kvrel_LIST_REL_val_approx]
+                  >- metis_tac[ksrel_sga]
+                  >- metis_tac[ksrel_ssgc_free]
+                  >- metis_tac[kvrel_EVERY_vsgc_free])
+              >- metis_tac[ssgc_free_preserved_SING']) >>
+          dsimp[krrel_err_rw] >> metis_tac[result_CASES])
       >- (imp_res_tac known_sing_EQ_E >> rveq >> fs[] >>
           simp[Once evaluate_CONS, pair_case_eq, result_case_eq] >>
           dsimp[] >> fs[krrel_err_rw] >>
-          metis_tac[result_CASES, pair_CASES]))
+          metis_tac[result_CASES, pair_CASES, known_better_definedg,
+                    kvrel_better_definedg]))
   >- (say "var" >>
       simp[evaluate_def, bool_case_eq, known_def] >>
-      rpt strip_tac >> fs[LIST_REL_EL_EQN])
+      rpt strip_tac >> fs[LIST_REL_EL_EQN] >> metis_tac[kvrel_approx_prefix])
   >- (say "if" >>
       simp[evaluate_def, pair_case_eq, bool_case_eq,
            result_case_eq, known_def] >> rpt strip_tac >> rveq >> fs[] >>
@@ -1553,24 +1626,93 @@ val known_correct0 = Q.prove(
       >- (imp_res_tac known_sing_EQ_E >> rveq >> fs[] >> rveq >>
           imp_res_tac evaluate_SING >> rveq >> fs[] >> rveq >>
           simp[evaluate_def] >> sel_ihpc last >> simp[] >> fs[] >>
-          disch_then irule >> simp[] >- metis_tac[ssgc_free_preserved_SING'] >>
-          metis_tac[kca_sing_sga])
+          qcase_tac `LIST_REL (kvrel eas g0) env1 env2` >>
+          qcase_tac `known [exp1] as g0 = ([(exp2,apx1)], g1)` >>
+          qcase_tac `evaluate ([exp1],env1,s01) = (Rval [Boolv T], s11)` >>
+          qcase_tac `evaluate ([exp2],env2,s02) = (Rval [Boolv T], s12)` >>
+          disch_then (qspecl_then [`env2`, `s12`, `eas`] mp_tac) >> impl_tac
+          >- (simp[] >> rpt conj_tac
+              >- (irule LIST_REL_mono >> qexists_tac `kvrel eas g0` >>
+                  simp[] >>
+                  metis_tac[kvrel_better_definedg, known_better_definedg])
+              >- (qpat_assum `known [exp1] _ _ = _`
+                    (mp_tac o MATCH_MP (GEN_ALL kca_sing_sga)) >> simp[] >>
+                  strip_tac >> sel_ihpc last >> reverse impl_tac
+                  >- metis_tac[ksrel_sga] >> simp[] >> rpt strip_tac
+                  >- metis_tac[kvrel_LIST_REL_val_approx]
+                  >- metis_tac[ksrel_sga]
+                  >- metis_tac[ksrel_ssgc_free]
+                  >- metis_tac[kvrel_EVERY_vsgc_free])
+              >- metis_tac[ssgc_free_preserved_SING']) >>
+          strip_tac >> simp[] >>
+          metis_tac[known_better_definedg, krrel_better_definedg])
       >- (imp_res_tac known_sing_EQ_E >> rveq >> fs[] >> rveq >>
-          imp_res_tac evaluate_SING >> rveq >> fs[] >> rveq >> strip_tac >>
-          simp[evaluate_def] >> sel_ihpc last >> simp[] >>
-          disch_then irule >- metis_tac[ssgc_free_preserved_SING] >>
-          irule state_approx_better_definedg >>
-          imp_res_tac known_better_definedg >>
-          metis_tac[kca_sing_sga])
+          imp_res_tac evaluate_SING >> rveq >> fs[] >> rveq >>
+          simp[evaluate_def] >> sel_ihpc last >> simp[] >> fs[] >>
+          qcase_tac `LIST_REL (kvrel eas g0) env1 env2` >>
+          qcase_tac `known [exp1] as g0 = ([(exp2,apx1)], g1)` >>
+          qcase_tac `evaluate ([exp1],env1,s01) = (Rval [Boolv F], s11)` >>
+          qcase_tac `evaluate ([exp2],env2,s02) = (Rval [Boolv F], s12)` >>
+          disch_then (qspecl_then [`env2`, `s12`, `eas`] mp_tac) >> impl_tac
+          >- (simp[] >> rpt conj_tac
+              >- (irule LIST_REL_mono >> qexists_tac `kvrel eas g0` >>
+                  simp[] >>
+                  metis_tac[kvrel_better_definedg, known_better_definedg,
+                            better_definedg_trans])
+              >- (qpat_assum `known [exp1] _ _ = _`
+                    (mp_tac o MATCH_MP (GEN_ALL kca_sing_sga)) >> simp[] >>
+                  strip_tac >> sel_ihpc last >> reverse impl_tac
+                  >- metis_tac[ksrel_sga, known_better_definedg,
+                               state_approx_better_definedg] >>
+                  simp[] >> rpt strip_tac
+                  >- metis_tac[kvrel_LIST_REL_val_approx]
+                  >- metis_tac[ksrel_sga]
+                  >- metis_tac[ksrel_ssgc_free]
+                  >- metis_tac[kvrel_EVERY_vsgc_free])
+              >- metis_tac[ssgc_free_preserved_SING']) >>
+          strip_tac >> simp[])
       >- (imp_res_tac known_sing_EQ_E >> rveq >> fs[] >> rveq >>
-          simp[evaluate_def]))
+          imp_res_tac evaluate_SING >> rveq >> fs[] >> rveq >>
+          simp[evaluate_def] >> rw[] >> fs[])
+      >- (imp_res_tac known_sing_EQ_E >> rveq >> fs[] >> rveq >>
+          simp[evaluate_def, pair_case_eq, result_case_eq, bool_case_eq] >>
+          fs[krrel_err_rw] >- (dsimp[] >> metis_tac[result_CASES, pair_CASES])>>
+          metis_tac[kvrel_better_definedg, known_better_definedg]))
   >- (say "let" >>
       simp[evaluate_def, pair_case_eq, result_case_eq] >>
       rpt strip_tac >> rveq >> fs[known_def] >>
-      rpt (pairarg_tac >> fs[]) >> rveq >> fs[] >> nailIH
-      >- (strip_tac >> simp[evaluate_def] >>
-          imp_res_tac known_sing_EQ_E >> rveq >> fs[] >> rveq >>
-          sel_ihpc last >> simp[] >> disch_then MATCH_MP_TAC >>
+      rpt (pairarg_tac >> fs[]) >> rveq >> fs[] >> nailIHx strip_assume_tac >>
+      simp[evaluate_def]
+      >- (imp_res_tac known_sing_EQ_E >> rveq >> fs[] >> rveq >>
+          sel_ihpc last >> simp[] >>
+          qcase_tac `evaluate (MAP FST alist2, env2, s02) = (Rval vs2, s12)` >>
+          qcase_tac `known exps1 as g0 = (alist2, g1)` >>
+          qcase_tac `evaluate (exps1,env1,s01) = (Rval vs1, s11)` >>
+          qcase_tac
+            `known [exp1] (MAP SND alist2 ++ as) g1 = ([(exp2,a2)], g2)` >>
+          disch_then (qspecl_then [`vs2 ++ env2`, `s12`, `as`] mp_tac) >>
+          simp[] >>
+          impl_tac
+          >- (rpt conj_tac
+              >- (irule EVERY2_APPEND_suff >> simp[] >>
+                  qspecl_then [`exps1`, `as`, `g0`, `alist2`, `g1`] mp_tac
+                              known_correct_approx >> simp[] >>
+                  disch_then (qspecl_then [`env2`, `s02`, `s12`, `Rval vs2`]
+                                          mp_tac) >> simp[] >> impl_tac
+                  >- (rpt conj_tac
+                      >- metis_tac [kvrel_LIST_REL_val_approx]
+                      >- metis_tac [ksrel_sga]
+                      >- metis_tac [ksrel_ssgc_free]
+                      >- metis_tac [kvrel_EVERY_vsgc_free]) >>
+                  metis_tac[kvrel_LIST_REL_val_approx])
+              >- (qspecl_then [`exps1`, `env1`, `s01`, `Rval vs1`, `s11`]
+                              mp_tac ssgc_evaluate >> simp[])
+
+metis_tac[kvrel_EVERY_vsgc_free]
+
+
+
+disch_then MATCH_MP_TAC >>
           qcase_tac `evaluate (MAP FST al1,env,s0) = (Rval vs, s1)` >>
           qcase_tac `evaluate ([bod], vs ++ env, s1) = (res,ss)` >>
           qcase_tac `known [bod] (MAP SND al1 ++ as) g1 = ([(bod',ba)], g)` >>
